updates

intermediate/Veritas.Intermediate.Verify.fst
@@ -1,6 +1,20 @@
 module Veritas.Intermediate.Verify
 open FStar.Classical
 
+(* initial epoch hashes - all hashes initialized to 0 (empty_hash_value) *)
+let init_epoch_hashes: epoch_hashes = fun e -> empty_hash_value
+
+(* update the hash of an epoch *)
+let upd_epoch_hash (ep2h: epoch_hashes) (ep: epoch) (e: ms_hashfn_dom): epoch_hashes =
+  (* previous hash of epoch ep *)
+  let h' = ep2h ep in
+  (* updated hash of epoch ep *)
+  let h = ms_hashfn_upd e h' in
+  fun ep' -> if ep = ep'
+          then h
+          else ep2h ep'
+
+
 #push-options "--z3rlimit_factor 2"
 
 let vaddm #vcfg (s:slot_id vcfg) (r:record) (s':slot_id vcfg) (vs: vtls vcfg {Valid? vs}):
