intermediate/Veritas.Intermediate.Thread.fsti
@@ -33,10 +33,10 @@ let index #vcfg (tl: thread_id_logS vcfg) (i:tl_idx tl): logS_entry _ =
 let prefix #vcfg (tl: thread_id_logS vcfg) (i:nat{i <= length tl}): thread_id_logS _ =
   (thread_id_of tl), (SA.prefix (logS_of tl) i)
 
-let init_store vcfg (tid:thread_id): vstore _ = 
+let init_store vcfg (tid:thread_id): vstore _ =
   let st = empty_store vcfg in
-  if tid = 0 then 
-    madd_to_store_root st 0 (init_value Root) 
+  if tid = 0 then
+    madd_to_store_root st 0 (init_value Root)
   else
     st
 
@@ -54,7 +54,7 @@ let verify #vcfg (tl:thread_id_logS vcfg): vtls _ =
   let vs = IntV.init_thread_state tid st in
   IntV.verify vs l
 
-let verifiable #vcfg (tl:thread_id_logS vcfg) = 
+let verifiable #vcfg (tl:thread_id_logS vcfg) =
   IntV.Valid? (verify tl)
 
 let verifiable_log vcfg = tl:thread_id_logS vcfg{verifiable tl}
@@ -71,7 +71,7 @@ let clock #vcfg (tl:verifiable_log vcfg) (i:tl_idx tl): timestamp =
 
 (* get the blum add element from an index *)
 let blum_add_elem #vcfg (e:logS_entry vcfg {is_blum_add e}):
-  ms_hashfn_dom = 
+  ms_hashfn_dom =
   match e with
   | AddB_S s r t j -> MHDom r t j
 
@@ -90,9 +90,12 @@ val lemma_add_seq_inv (#vcfg:_) (tl: verifiable_log vcfg) (i: seq_index tl{is_bl
   Lemma (ensures (add_seq_inv_map tl (add_seq_map tl i) = i))
         [SMTPat (add_seq_map tl i)]
 
-let hadd #vcfg (tl: verifiable_log vcfg): ms_hash_value = 
-  Valid?.hadd (verify tl)
-
+(* aggregated hash upto current epoch *)
+let hadd #vcfg (tl: verifiable_log vcfg): ms_hash_value =
+  let vs = verify tl in
+  match vs with
+  | Valid _ _ (MkTimestamp ep _) ha _ ->
+    IntV.aggr_epoch_hashes_upto ha ep
 
 (* the verifier state after processing i entries *)
 let state_at #vcfg (tl: verifiable_log vcfg) (i:nat{i <= length tl}): st:vtls _{Valid? st} =
@@ -100,15 +103,15 @@ let state_at #vcfg (tl: verifiable_log vcfg) (i:nat{i <= length tl}): st:vtls _{
 
 val lemma_state_transition (#vcfg:_)
                            (tl: verifiable_log vcfg)
-                           (i: tl_idx tl): 
-  Lemma (state_at tl (i + 1) == 
+                           (i: tl_idx tl):
+  Lemma (state_at tl (i + 1) ==
          verify_step (state_at tl i) (index tl i))
 
 val lemma_hadd_correct (#vcfg:_) (tl: verifiable_log vcfg):
   Lemma (ensures (hadd tl = ms_hashfn (blum_add_seq tl)))
         [SMTPat (verifiable tl)]
 
-let blum_evict_elem (#vcfg:_) (tl: verifiable_log vcfg) (i:seq_index tl{is_evict_to_blum (index tl i)}): ms_hashfn_dom = 
+let blum_evict_elem (#vcfg:_) (tl: verifiable_log vcfg) (i:seq_index tl{is_evict_to_blum (index tl i)}): ms_hashfn_dom =
   let (tid, _) = tl in
   let tli = prefix tl i in
   let tli' = prefix tl (i + 1) in
@@ -118,14 +121,17 @@ let blum_evict_elem (#vcfg:_) (tl: verifiable_log vcfg) (i:seq_index tl{is_evict
 
 val blum_evict_seq (#vcfg:_) (tl: verifiable_log vcfg): S.seq ms_hashfn_dom
 
-let hevict #vcfg (tl: verifiable_log vcfg): ms_hash_value = 
-  Valid?.hevict (verify tl)
+let hevict #vcfg (tl: verifiable_log vcfg): ms_hash_value =
+  let vs = verify tl in
+  match vs with
+  | Valid _ _ (MkTimestamp ep _) _ he ->
+    IntV.aggr_epoch_hashes_upto he ep
 
 val lemma_hevict_correct (#vcfg:_) (tl: verifiable_log vcfg):
   Lemma (hevict tl = ms_hashfn (blum_evict_seq tl))
 
 val evict_seq_map (#vcfg:_) (tl: verifiable_log vcfg) (i: seq_index tl{is_evict_to_blum (index tl i)}):
-  (j: SA.seq_index (blum_evict_seq tl) {S.index (blum_evict_seq tl) j = 
+  (j: SA.seq_index (blum_evict_seq tl) {S.index (blum_evict_seq tl) j =
                                         blum_evict_elem tl i})
 
 val evict_seq_inv_map (#vcfg:_) (tl: verifiable_log vcfg) (j: SA.seq_index (blum_evict_seq tl)):
@@ -137,12 +143,12 @@ val lemma_evict_seq_inv (#vcfg:_) (tl: verifiable_log vcfg) (i: seq_index tl{is_
   Lemma (ensures (evict_seq_inv_map tl (evict_seq_map tl i) = i))
         [SMTPat (evict_seq_map tl i)]
 
-val lemma_blum_evict_elem_prefix (#vcfg:_) (tl: verifiable_log vcfg) (i: nat{i <= length tl}) 
+val lemma_blum_evict_elem_prefix (#vcfg:_) (tl: verifiable_log vcfg) (i: nat{i <= length tl})
   (j: nat{j < i && is_evict_to_blum (index tl j)}):
   Lemma (blum_evict_elem tl j = blum_evict_elem (prefix tl i) j)
 
 val lemma_add_clock (#vcfg:_) (tl: verifiable_log vcfg) (i: seq_index tl{is_blum_add (index tl i)}):
-  Lemma (timestamp_of (blum_add_elem (index tl i)) `ts_lt`  clock tl i) 
+  Lemma (timestamp_of (blum_add_elem (index tl i)) `ts_lt`  clock tl i)
 
 val lemma_evict_clock (#vcfg:_) (tl: verifiable_log vcfg) (i: seq_index tl{is_evict_to_blum (index tl i)}):
   Lemma (timestamp_of (blum_evict_elem tl i) = clock tl i)
@@ -155,4 +161,3 @@ val lemma_clock_monotonic (#vcfg:_) (tl: verifiable_log vcfg) (i:seq_index tl) (
 
 val lemma_evict_elem_unique (#vcfg:_) (tl: verifiable_log vcfg) (i1 i2: SA.seq_index (blum_evict_seq tl)):
   Lemma (i1 <> i2 ==> S.index (blum_evict_seq tl) i1 <> S.index (blum_evict_seq tl) i2)
-
